   x + y = 24
-<ins>2x - y = -6</ins>

   2x + 2y = 48
-<ins>2x - y = -6</ins>
3y = 54
y = 18


x + y = 24
x + 18 = 24
x = 6


x,y = 6, 18

-(3x/4 - 1/2) = 1/2
3x/4 - 1/2 = -1/2
3x/4 = 0
x = 0


```
    ┌      ┐
a = │-1   9│
    │ 2   4│
    └      ┘
```
```
    ┌      ┐
b = │ 0  -6│
    │ 8  10│
    └      ┘
```
-2A + 1/2B = 
```
      ┌      ┐
-2a = │ 2 -18│
      │-4  -8│
      └      ┘
```
```
       ┌      ┐
1/2b = │ 0  -3│
       │ 4   5│
       └      ┘
```

-2A + 1/2B = 
```
             ┌       ┐
-2a + 1/2b = │ 2  -21│
             │ 0   -3│
             └       ┘
```
AB = 
```
    ┌      ┐
a = │-1   9│
    │ 2   4│
    └      ┘
```
```
    ┌      ┐
b = │ 0  -6│
    │ 8  10│
    └      ┘
```
2x2x2x2

r1c1 






DB = 
```
    ┌      ┐
d = │-2  -4│
    │ 9   1│
    └      ┘
```
```
    ┌      ┐
b = │ 5   6│
    │-9  -3│
    └      ┘
```
r1c1 2(5)-4(-9)
r1c2 2(6)-4(-3)
r2c1 9(5)+1(-9)
r2c2 9(6)+ 1(-3)

5 is not possible 

6 answer is
```
    ┌              ┐
b = │ -36 -14   -54│
    │  20         │
    └      ┘
```




w - (-9) = -15
w + 9 = -15
w = -24

x - (-2x) = -15
x + 2x = -15
3x = -15
x = -5

y - 6 = 8
5 - z = -10
-z = -15
z =15

-3(w) -1 = -1 

-3(4) + x + y = 7
-3(y)+2y = 8 
y = 8

-3(4) + x + 8 = 7


$$
\begin{bmatrix}  
1 & 2 & 3\\  
a & b & c  
\end{bmatrix}
$$